messageInvariantPrototypes/ringLeaderElection/automate/applicationProof.dfy
@@ -96,7 +96,18 @@ lemma ChordDominatesInductive(c: Constants, v: Variables, v': Variables)
   requires Next(c, v, v')
   ensures ChordDominates(c, v')
 {
-  VariableNextProperties(c, v, v');
+  forall i:int, src:nat, dst:nat, mid:nat | 
+      && v'.ValidHistoryIdx(i)
+      && c.ValidIdx(src)
+      && c.ValidIdx(dst)
+      && c.ValidIdx(mid)
+      && v'.History(i).hosts[dst].highestHeard == c.hostConstants[src].hostId
+      && Between(src, mid, dst)
+  ensures
+      c.hostConstants[mid].hostId < c.hostConstants[src].hostId
+  {
+    VariableNextProperties(c, v, v');
+  }
 }
 }  // end module RingLeaderElectionProof
 
